src/UnfolderTests.v
@@ -80,47 +80,47 @@ Module Make (B : Heap).
     Definition hints_tt : U.hints.
       prepare tt tt.
     Defined.
-    Print hints_tt.
+(*    Print hints_tt. *)
 
     Definition hints_emp : U.hints.
       prepare Hemp Hemp.
     Defined.
-    Print hints_emp.
+(*    Print hints_emp. *)
 
     Definition hints_Hf : U.hints.
       prepare Hf Hemp.
     Defined.
-    Print hints_Hf.
+(*    Print hints_Hf. *)
 
     Definition hints_Hh : U.hints.
       prepare (Hemp, Hf) (Hemp, Hf, Hh).
     Defined.
-    Print hints_Hh.
+(*    Print hints_Hh. *)
 
     Definition hints_Hf0 : U.hints.
       prepare Hf0 tt.
     Defined.
-    Print hints_Hf0.
+(*    Print hints_Hf0. *)
 
     Definition hints_glom : U.hints.
       prepare (Hemp, Hf, Hh, Hf0) (Hemp, Hf0, tt).
     Defined.
-    Print hints_glom.
+(*    Print hints_glom. *)
 
     Definition hints_Hh0 : U.hints.
       prepare Hh0 tt.
     Defined.
-    Print hints_Hh0.
+(*    Print hints_Hh0. *)
 
     Definition hints_Hf1 : U.hints.
       prepare Hf1 tt.
     Defined.
-    Print hints_Hf1.
+(*    Print hints_Hf1. *)
 
     Definition hints_Hh1 : U.hints.
       prepare Hh1 tt.
     Defined.
-    Print hints_Hh1.
+(*    Print hints_Hh1. *)
 
 
     (** * Simplifying some goals *)
@@ -138,7 +138,7 @@ Module Make (B : Heap).
         Types Functions PcType StateType SFunctions Hints Lhs Rhs
         equiv_dec ExprUnify.exprUnifyArgs ExprUnify.fold_left_2_opt
         ExprUnify.exprUnify exprSubstU sheapSubstU EqDec_tvar tvar_rec tvar_rect sumbool_rec sumbool_rect
-        eq_rec_r eq_rec eq_rect eq_sym f_equal ExprUnify.get_Eq defaultType
+        eq_rec_r eq_rec eq_rect eq_sym f_equal ExprUnify.get_Eq 
         nth_error value error Eq liftExpr DepList.seq_dec ExprUnify.Subst_lookup SHeap_empty
         exists_subst ExprUnify.env_of_Subst fst snd tvarD sexprD
         Impl sheapD starred fold_right applyD
